
# Phase space:

A state of a classical system at some time $t$ is a complete set of data that fully specifies future evolution of the system. The [[Calculus of variations#Euler-Lagrange equations|Euler-Lagrange]] equations are $n$ second order equations in $u$ generalised coordinates. These need $2n$ constants to be fully determined.

Phase space is defined as the set of all possible states for a system at a given time. This is analogous to the definition of [[Calculus of variations#Configuration space and generalised coordinates|configuration space]], however allowing the inclusion of any relevant information in a state. This results in:$$\Huge \dim(\text{Phase space})=2\dim(\text{Configuration space})$$For example, a particle moving in one dimension can be parametrised with $x(t)$ and $\dot x(t)$. The configuration space is $\{x(t)\}$ whereas phase space is $\{x(t),\dot x(t)\}$. This example can be extended to a particle moving in $\Re^d$, where the phase space would become $\Re^{2d}$.

The Hamiltonian Formalism is the study of dynamics in phase space parametrised by [[Calculus of variations#Configuration space and generalised coordinates|generalised coordinates]] $\underline q_i$ and their associated [[Lagrangians for classical mechanics#Ignorable coordinates and Conservation of momentum|generalised momenta]] $p_i$. The fundamental step here is to invert the defining relations for $p_i$:$$\Huge p_i=\frac{\partial L}{\partial \underline q_i}(\underline q,\dot{\underline q})\implies \underline{\dot q_i}(\underline q,\underline p)$$Where we solve the equations generated by the LHS to find $\underline{\dot q_i}$ in terms of $\underline q$ and $\underline p$.

The simplest example for this is considering a massive particle moving in $\Re$. Then we have:$$\Huge L=\frac{1}{2}m\dot x^2\implies p=\frac{\partial L}{\partial\dot x}=m\dot x\implies \dot x=\frac{p}{m}\implies L=\frac{1}{2}\frac{p^2}{m}$$

# Poisson bracket:

Given two functions $f(\underline q,\underline p),g(\underline q,\underline p)$ in phase space, we define the Poisson bracket:$$\Huge \{f,g\}:=\sum_{i=1}^n\left(\frac{\partial f}{\partial q_i}\frac{\partial g}{\partial p_i}-\frac{\partial f}{\partial p_i}\frac{\partial g}{\partial q_i}\right)$$Note that $\frac{\partial q_i}{\partial p_j}=\frac{\partial p_j}{\partial q_i}=0$, that is $\underline p$ and $\underline q$ are held constant. Taking $f=g=q_1$ we see:$$\Huge\{q_1,q_1\}=\sum_{i=1}^n\left(\frac{\partial q_1}{\partial q_i}\frac{\partial q_1}{\partial p_i}-\frac{\partial q_1}{\partial p_i}\frac{\partial q_1}{\partial q_i}\right)=0$$Since, by definition, $\frac{\partial q_1}{\partial p_i}=0$. This holds for any two coordinates or two generalised momenta:$$\Huge \{q_i,q_j\}=\{p_i,p_j\}=0$$We can then compute:$$\Huge \{q_i,p_j\}=\sum_{k=1}^n\left(\frac{\partial q_i}{\partial q_k}\frac{\partial p_j}{\partial p_k}-\frac{\partial q_i}{\partial p_k}\frac{\partial p_j}{\partial q_k}\right)=\sum_{k=1}^n\frac{\partial q_i}{\partial q_k}\frac{\partial p_j}{\partial p_k}=\delta_{ij}$$
One can prove the following properties of the Poisson bracket:
> $\{f,g\}=-\{g,f\}$, antisymmetric
> $\{\alpha f+\beta h,g\}=\alpha\{f,g\}+\beta\{h,g\}$ and $\{f,\alpha g+\beta h\}=\alpha\{f,g\}+\beta\{f,h\}$ bilinear on both terms
> $\{f,gh\}=\{f,g\}h+\{f,h\}g$, Leibniz identity
> $\{\{f,g\},h\}+\{\{h,f\},g\}+\{\{g,h\},f\}=0$, Jacobi identity

# Hamiltonian flows:

We define $\mathcal{F}=\{f:P\mapsto\Re\}$, the set of all functions from a Phase space to the real line. We also define the Hamiltonian flow operator $\Phi_f^{(\epsilon)}:\mathcal{F}\mapsto\mathcal{F}$:$$\Huge\Phi_{f}^{(\epsilon)}(g)=g+\epsilon\{g,f\}+\mathcal{O}(\epsilon^2)$$Note that when we take $g=\underline q_i$ or $g=p_i$:$$\Huge\begin{align}
\Phi_f^{(\epsilon)}(\underline q_i)&=\underline q_i+\epsilon\{\underline q_i,f\}+\mathcal{O}(\epsilon^2)\\
\Phi_f^{(\epsilon)}(p_i)&=p_i+\epsilon\{p_i,f\}+\mathcal{O}(\epsilon^2)
\end{align}$$These can be simplified since:$$\Huge\begin{align}
\{\underline q_i,f(\underline q,p)\}&=\sum_{k=1}^n\left(\frac{\partial \underline q_i}{\partial \underline q_k}\frac{\partial f}{\partial p_k}-\frac{\partial \underline q_i}{\partial p_k}\frac{\partial f}{\partial \underline q_k}\right)=\frac{\partial f}{\partial p_i}\\
\{p_i,f(\underline q,p)\}&=-\frac{\partial f}{\partial \underline q_i}
\end{align}$$So we get:$$\Huge\begin{align}
\Phi_f^{(\epsilon)}(\underline q_i)&=\underline q_i+\epsilon\frac{\partial f}{\partial p_i}+\mathcal{O}(\epsilon^2)\\
\Phi_f^{(\epsilon)}(p_i)&=p_i-\epsilon\frac{\partial f}{\partial \underline q_i}+\mathcal{O}(\epsilon^2)
\end{align}$$One can interpret the Hamiltonian flow through Taylor expansion in $\epsilon$:$$\large\begin{align}
\Phi_f^{(\epsilon)}(g)&=g(\underline q_1+\{\underline q_1,f\},\dots,\underline q_n+\{\underline q_n,f\},p_1+\{p_1,f\},\dots,p_n+\{p_n,f\})\\
&=g(\underline q,p)+\epsilon\sum_{i=1}^n\left(\frac{\partial g}{\partial \underline q_i}\{\underline q_i,f\}+\frac{\partial f}{\partial p_i}\{p_i,f\}\right)\\
&=g(\underline q,p)+\epsilon\sum_{i=1}^n\left(\frac{\partial g}{\partial \underline q_i}\frac{\partial f}{\partial p_i}-\frac{\partial g}{\partial p_i}\frac{\partial f}{\partial \underline q_i}\right)\\
&=g(\underline q,p)+\epsilon\{g,f\}+\mathcal{O}(\epsilon^2)
\end{align}$$So we observe that these different methods of interpreting $\Phi$ result in the same outcome.

Take for example a particle moving in one dimension. In this case, $P$ is parametrised by $\{x(t),\dot x(t)\}$:$$\Huge\begin{align}
\Phi_p^{(\epsilon)}(f)&=f+\epsilon\{f,p\}\\
&=f-\epsilon\{p,f\}\\
&=f+\epsilon\frac{\partial f}{\partial x}\\
\Phi_p^{(\epsilon)}(x)&=x+\epsilon\frac{\partial x}{\partial x}\\
&=x+\epsilon
\end{align}$$We can illustrate this as such:![[constant shift]]

We aim to prove that the [[Symmetries, Noether's theorem, and conservation laws#Noether's theorem|Noether charge]] for a transformation generates said transformation. Assume we have $\underline q_i\rightarrow\underline q_i+\epsilon a_i(\underline q)$ and define:$$\Huge Q(\underline q,\dot{\underline q})=\left(\sum_{i=1}^na_i\frac{\partial L}{\partial \dot{\underline q}}\right)-F(\underline q)$$We can formalise this in Hamiltonian variables:$$\Huge Q(\underline q,p)=\left(\sum_{i=1}^na_i(\underline q)p_i\right)-F(\underline q)$$Now we aim to show that this charge generates the given transformation. To do this, observe the Hamiltonian flow over $Q$ on the coordinates $\underline q_i$:$$\Huge\begin{align}
\Phi_Q^{(\epsilon)}(\underline q_i)&=\underline q_i+\epsilon\{\underline q_i,Q\}\\
&=\underline q_i+\epsilon\left(\sum_{k=1}^n\{\underline q_i,a_kp_k\}+\{\underline q_i,F(\underline q)\}\right)\\
&=\underline q_i+\epsilon\left(\sum_{k=1}^np_k\{\underline q_i,a_k\}+a_k\{\underline q_i,p_k\}+0\right)\\
&=\underline q_i+\epsilon\left(\sum_{k=1}^n0+a_k\delta_{ik}\right)\\
&=\underline q_i+\epsilon(a_i)
\end{align}$$So we get the correct transformation as required.