
# Canonical kinetic terms

Restricting to [[Calculus of variations#Action principle|Lagrangians]] of the form:$$\Huge L=\frac{1}{2}\sum_{i=1}^n\dot q_i^2-V(\underline q)$$The kinetic term represented in the sum is known as a canonical kinetic term. Assuming there is a stationary point of $V(\underline q)$ at $\underline q=0$. Note if there is not a stationary point here, one can introduce the transformation $\underline q'=\underline q-\underline a$ to move to the required point. Now by [[Taylor series|Taylor expanding]] about $\underline q=0$:$$\Huge V(\underline q)=V(\underline 0)+\sum_{i=1}^n \underline q_i \frac{\partial V}{\partial \underline q_i}\vert_0+\frac{1}{2}\sum_{i,j=1}^n\underline q_i\underline q_j\frac{\partial^2V}{\partial\underline q_i\partial\underline q_j}\vert_0+\dots$$Now define:$$\Huge A_{ij}=\frac{\partial^2V}{\partial\underline q_i\partial\underline q_j}\vert_0$$Note that $A$ is symmetric. Then we can approximate the Lagrangian:$$\Huge L_{\text{approx}}=\frac{1}{2}\sum_{i=1}^n\underline{\dot q}_i^2-\frac{1}{2}\sum_{i,j=1}^n\underline q_iA_{ij}\underline q_j-V(0)$$The approximate [[Calculus of variations#Euler-Lagrange equations|Euler-Lagrange]] equations then become:$$\Huge\begin{align}
\frac{d}{dt}(\frac{\partial L}{\partial \underline{\dot q}_k})-\frac{\partial L_{\text{approx}}}{\partial \underline q_k}&=0\\
\ddot{\underline q}_k+\frac{1}{2}\left(\sum_{j=1}^nA_{kj}\underline q_j+\sum_{i=1}^n\underline q_iA_{ik}\right)&=\\
\ddot{\underline q}_k+\frac{1}{2}\left(\sum_{j=1}^nA_{kj}\underline q_j+\sum_{i=1}^nA_{ki}\underline q_i\right)&=\\
\ddot{\underline q}_k+\sum_{i=1}^nA_{ki}\underline q_i&=\\\ddot{\underline q}_k+A\underline q&=
\end{align}$$Since $A$ is a symmetric matrix, there must exist a matrix $O$ such that:$$\Huge D=OAO^{-1}$$Is [[Eigenvalues, Eigenvectors, and Diagonalisation#Diagonalisation|diagonal]]. Let $\underline q'=O\underline q$, that is $\underline q=O_{-1}\underline q'$. Then the approximate Euler-Lagrange equations become:$$\Huge O^{-1}\ddot{\underline q}'+AO^{-1}\underline q'=0\implies\ddot{\underline q}'+OAO^{-1}\underline q'=0\implies\ddot{\underline q}'+D\underline q'=0$$That is:$$\Huge \begin{pmatrix}\ddot q_1'\\\vdots\\\ddot q_n'\end{pmatrix}+\begin{pmatrix}\lambda_1&\dots&0\\\vdots&\ddots&\vdots\\0&\dots&\lambda_n\end{pmatrix}\begin{pmatrix}q_1'\\\vdots\\q_n'\end{pmatrix}=0$$This gives $n$ one dimensional problems of the form:$$\Huge \ddot q_i'+\lambda_iq_i'=0$$For all $i\in\{1,\dots,n\}$. Define $\underline v^{(i)}$ such that:$$\Huge A\underline v^{(i)}=\lambda^{(i)}\underline v^{(i)}$$Take the ansatz:$$\Huge \underline q^{(i)}(t)=\underline v^{(i)}f^{(i)}(t)\implies\underline{\ddot q}^{(i)}+A\underline q^{(i)}=\underline v^{(i)}\ddot f^{(i)}(t)+(A\underline v^{(i)})f^{(i)}(t)$$By definition, $\underline v$ is an [[Eigenvalues, Eigenvectors, and Diagonalisation#Eigenspaces|eigenvector]] so we can write the above as:$$\Huge\begin{align}
\underline{\ddot q}^{(i)}+A\underline q^{(i)}&=\underline v^{(i)}\ddot f^{(i)}(t)+\lambda^{(i)}\underline v^{(i)}f^{(i)}(t)\\&=\underline v^{(i)}(\ddot f^{(i)}(t)+\lambda^{(i)}f^{(i)}(t))=0
\end{align}$$Which implies the bracketed term $\ddot f^{(i)}(t)+\lambda^{(i)}f^{(i)}(t)$ equal to $0$. Writing this with a differential operator:$$\Huge \left(\frac{d^2}{dt^2}+\lambda^{(i)}\right)f^{(i)}(t)=0$$We then get cases for $\lambda^{(i)}<0,\lambda^{(i)}=0,\lambda^{(i)}>0$:$$\Huge f^{(i)}(t)=\begin{cases}\alpha^{(i)}\cos(t\sqrt{\lambda^{(i)}})+\beta^{(i)}\sin(t\sqrt{\lambda^{(i)}})&\text{for }\lambda^{(i)}>0\\
C^{(i)}t+D^{(i)}&\text{for }\lambda^{(i)}=0\\ 
\alpha^{(i)}\cosh(t\sqrt{-\lambda^{(i)}})+\beta^{(i)}\sinh(t\sqrt{-\lambda^{(i)}})&\text{for }\lambda^{(i)}<0
\end{cases}$$The case where $\lambda^{(i)}>0$ is called a normal mode, $\lambda^{(i)}=0$ is the zero mode, and $\lambda^{(i)}<0$ is called an instability. This solution can be written as a single equation:$$\Huge\begin{align}
\underline q(t)=&\sum_{i:\lambda^{(i)}>0}\underline v^{(i)}(\alpha^{(i)}\cos(t\sqrt{\lambda^{(i)}})+\beta^{(i)}\sin(t\sqrt{\lambda^{(i)}}))\\
&+\sum_{i:\lambda^{(i)}=0}\underline v^{(i)}(C^{(i)}t+D^{(i)})\\
&+\sum_{i:\lambda^{(i)}<0}\underline v^{(i)}(\alpha^{(i)}\cosh(t\sqrt{-\lambda^{(i)}})+\beta^{(i)}\sinh(t\sqrt{-\lambda^{(i)}}))
\end{align}$$