[[Fourier Series]] can be thought of as frequency analysis of periodic functions, while the Fourier tranform can be thought of as frequency analysis of non-periodic functions. The fourier series of a function with period $2\pi$ can be written as:$$\Huge f(x)=\sum_{n=-\infty}^\infty d_ne^{inx}$$In the fourier series, coefficients $a_n,b_n$ tell you how much angular frequence $n$ is in $f(x)$. One can write $R=\sqrt{a_n^2+b_n^2}$ and $\alpha=\tan^{-1}(\frac{a_n}{b_n})$, allowing the summand in the fourier series to be written as:$$\Huge a_n\cos(nx)+b_n\sin(nx)=R\sin(nx+\alpha)$$Large $n$ corresponts to high frequencies, corresponding to small wavelength and therefore finer detail in a fourier series. The Fourier series for a function $f(x)$ with period $2\pi M$ can be written as:$$\Huge f(x)=\frac{a_0}{2}+\sum_{n=1}^\infty a_n\cos\left(\frac{nx}{M}\right)+b_n\sin\left(\frac{nx}{M}\right)=\sum_{n=-\infty}^\infty d_ne^{\frac{inx}{M}}$$If $M\to \infty$, then $f(x)$ will become non-periodic, however all frequencies will appear in the series. We then write:$$\Huge f(x)=\frac{1}{2\pi}\int_{-\infty}^\infty\tilde f(p)e^{ipx}dp$$Where $\tilde f(p)$ is the fourier transform of $f(x)$. Given $f(x)$, we aim to find coefficients $\tilde f(p)$. Let $f(x)$ be some non-periodic function, and define a periodic function $f_M(x)$ such that $f_M(x)=f(x),f_M(x+2\pi M)=f_M(x))$ on the interval $x\in\left[-\pi M,\pi M\right)$. Then for $f_M$ we write:$$\Huge f_M(x)=\sum_{-\infty}^\infty d_ne^{\frac{inx}{M}}$$Where:$$\Huge d_n=\frac{1}{2\pi M}\int_{-\pi M}^{\pi M}f_M(x)e^{-\frac{inx}{M}}dx=\frac{1}{2\pi M}\int_{-\pi M}^{\pi M}f(x)e^{-\frac{inx}{M}}dx$$Note that $d_n\to 0$ as $M\to \infty$, since there are more of them adding up to the same function. Let $\tilde f(\frac{n}{M})=2\pi Md_n$. This lets us rewrite the above as:$$\Huge \tilde f\left(\frac{n}{M}\right)=\int_{-\pi M}^{\pi M}f(x)e^{-\frac{inx}{M}}dx$$Now writing $p=\frac{n}{M}$ gives us:$$\Huge \tilde f(p)=\int_{-\pi M}^{\pi M}f(x)e^{-ipx}dx$$We can also rewrite the original series:$$\Huge f_M(x)=\frac{1}{2\pi M}\sum_{-\infty}^\infty\tilde f\left(\frac{n}{M}\right)e^{\frac{inx}{M}}=\frac{1}{2\pi}\sum_{-\infty}^\infty\tilde f(p)e^{ipx}\Delta p$$Where $\Delta p=\frac{1}{M}$, the difference between two neighbouring frequencies. Note that $\Delta p\to 0$ as $M\to\infty$ and:$$\Huge f_M(x)\to f(x)=\frac{1}{2\pi}\int_{-\infty}^\infty\tilde f(p)e^{ipx}dp$$Where $\tilde f(p)$ is given by:$$\Huge \tilde f(p)=\int_{-\infty}^\infty f(x)e^{-ipx}dx$$

# Properties:

## Linearity: 
If $f(x),g(x)$ have corresponding Fourier transforms $\tilde f(x),\tilde g(x)$, then $h(x)=\alpha f(x)+\beta g(x)$ has Fourier transform $\tilde h(x)=\alpha\tilde f(x)+\beta\tilde g(x)$, which comes from the linearity of the integral.

## Shift theorem: 
If $f(x)$ has Fourier transform $\tilde f(x)$, then $g(x)=f(x+a)$ has Fourier transform $\tilde g(p)=\tilde f(p)e^{ipa}$. Substituting $x'=x+a$ into the integral formula gives:$$\large \int_{-\infty}^\infty f(x+a)e^{-ipx}dx=\int_{-\infty}^\infty f(x')e^{-ip(x'-a)}dx'=e^{ipa}\int_{-\infty}^\infty f(x')e^{-ipa}dx'=e^{ipa}\tilde f(p)$$As required.

## Scaling theorem:
If $f(x)$ has Fourier transform $\tilde f(p)$, then the Fourier transform of $F(x)=f(bx)$ is given by:$$\Huge \tilde F(p)=\frac{1}{|b|}\tilde f\left(\frac{p}{b}\right)$$The proof is similar as above, substituting $x'=bx$. Both of the above theorems can be combined to define the Fourier transform of $F(x)=f(bx+a)$:$$\Huge \tilde F(p)=\frac{1}{|b|}\tilde f\left(\frac{p}{b}\right)e^{ipa}$$
## Even and odd functions:
If we denote the Fourier transform of an even function $f(x)$ as $\tilde f(p)$, then this will be an even function in $p$. Since this is an integral over all $x$, only the even part of the integrand contributes, so write:$$\small \tilde f(p)=\int_{-\infty}^\infty f(x)e^{-ipx}dx=\frac{1}{2}\int_{-\infty}^\infty f(x)e^{-ipx}+f(-x)e^{ipx}dx=\frac{1}{2}\int_{-\infty}^\infty f(x)(e^{-ipx}+e^{-ipx})dx=\frac{1}{2}(\tilde f(p)+\tilde f(-p))$$Implying that $\tilde f(p)=\tilde f(-p)$, a similar statement holds for odd functions $f(x)$.

## Fourier transform of derivatives:
If $f(x)$ has Fourier transform $\tilde f(p)$, then the derivative of $f$ has Fourier transform $ip\tilde f(p)$:$$\ \tilde f'(p)=\int_{-\infty}^\infty\frac{df}{dx}e^{-ipx}dx=[f(x)e^{-ipx}]_{-\infty}^\infty-\int_{-\infty}^\infty f(x)(ipe^{-ipx})dx=0+ip\int_{-\infty}^\infty f(x)e^{-ipx}=ip\tilde f(x)$$As required.

## Convolution theorem:
The convolution of two functions $f(x),g(x)$ is defined as:$$\Huge f\star g(x)=\int_{-\infty}^\infty f(t)g(x-t)dt$$Note that substituting $t'=x-t$, one can show that $f\star g(x)=g\star f(x)$. The convolution theorem states that if $\tilde f(p),\tilde g(p)$ are Fourier transforms of $f,g$ respectively, then the Fourier transform of their convolution is $\tilde f(p)\tilde g(p)$:$$ F(p)=\int_{-\infty}^\infty f\star g(x)e^{-ipx}dx=\int_{-\infty}^\infty\int _{-\infty}^\infty f(t)g(x-t)dt\,e^{-ipx}dx=\int_{-\infty}^\infty\int_{-\infty}^\infty f(t)g(x')dt\,e^{-ip(x'+t)}dx'$$$$\Huge \implies F(p)=\int_{-\infty}^\infty f(t)e^{-ipt}dt\,\,\int_{-\infty}^\infty g(x')e^{-ipx'}dx'=\tilde f(p)\tilde g(p)$$
# Examples:

Let $f(x)=e^{-x}$ for $x\geq0$ and $0$ otherwise, we can find the Fourier transform as follows:$$ \tilde f(p)=\int_{-\infty}^\infty f(x)e^{-ipx}=\int_0^\infty e^{-x}e^{-ipx}dx=\int_0^\infty e^{-(ip+1)x}dx=\left[-\frac{e^{-(ip+1)x}}{ip+1}\right]_0^\infty=\frac{1}{ip+1}$$More generally if $g(x)=e^{-bx}$ for $x\geq0$ and $0$ otherwise, we can use the scaling theorem to show that:$$\Huge \tilde g(p)=\frac{1}{b}f\left(\frac{p}{b}\right)=\frac{1}{b}\times\frac{1}{i\left(\frac{p}{b}+1\right)}=\frac{1}{ip+b}$$

Let $f(x)=e^{-x^2}$, then the Fourier transform is:$$\large \tilde f(p)=\int_{-\infty}^\infty e^{-x^2}e^{-ipx}dx=\int_{-\infty}^\infty e^{-(x+\frac{ip}{2})^2}e^{\frac{(ip)^2}{4}}dx=e^{-\frac{p^2}{4}}\int_{-\infty}^\infty e^{-x'^2}dx'=e^{-\frac{p^2}{4}}\sqrt{\pi}$$Letting $x'=x+\frac{ip}{2}$, and using the known result for the integral of a gaussian over the reals. Scaling and shift theorems can be used to find the Fourier transform if $f(x)=e^{-bx^2-cx}$ for $b>0$:$$\Huge \tilde f(p)=e^{-\frac{1}{4b}(p-ic)^2}\sqrt{\frac{\pi}{b}}$$
# Applications of Fourier Transforms to linear inhomogeneous ODEs:

Since the Fourier transform $\frac{dy}{dx}$ is $ip\tilde y$, differentiation in $x$-space corresponds to multiplication of $ip$ in $p$-space. Instead of directly solving an inhomogeneous linear ODE, one can find its Fourier transform, then divide by $ip$ to find the solution's Fourier transform, then taking the inverse Fourier transform to find the original solution. Take the example:$$\Huge \frac{dy}{dx}+3y=f(x)\mapsto(ip)\tilde y+3\tilde y=\tilde f(p)\implies\tilde y(p)=\frac{1}{ip+3}\tilde f(p)=\tilde f(p)\tilde g(p)$$Where $\tilde g(p)=\frac{1}{ip+3}$. We can use the convolution theorem here to say that $y(x)=f(x)\star g(x)$. We saw earlier that $\frac{1}{ip+b}$ is the Fourier transform of $e^{-bx}$ for $x\geq0$, so we can take $g(x)=e^{-3x}$:$$\Huge y(x)=\int_{-\infty}^\infty f(t)g(x-t)dt=\int_{-\infty}^xf(t)e^{-3(x-t)}dt=\frac{1}{e^{3x}}\int_{-\infty}^xf(t)e^{3t}dt$$
# Application of Fourier Transforms to PDEs:

Consider PDEs in two variables, of form $u(x,t)$. Taking the Fourier Transform with respect to $x$ gives:$$\Huge \tilde u(p,t)=\int_{-\infty}^\infty u(x,t)e^{-ipx}dx$$This transforms all partial derivatives of $x$ in a PDE into multiplication by $ip$:$$\Huge \tilde u_t(p,t)=\int_{-\infty}^\infty u_t(x,t)e^{-ipx}dx$$This method can transform these PDEs into ODEs involving only $t$ derivatives. Take for example $u_t-3u_x=-5u$ with $u(x,0)=R(x)$. Taking the FT gives:$$\Huge \tilde u_t-3(ip)\tilde u=-5\tilde u\implies\frac{\partial\tilde u}{\partial t}=(3ip-5)\tilde u\implies \tilde u=A(p)e^{(3ip-5)t}$$Where $A$ is some function of $p$. Putting $t=0$ gives:$$\Huge \tilde u(p,0)=\int_{-\infty}^\infty u(x,0)e^{-ipx}dx=\int_{-\infty}^\infty R(x)e^{-ipx}dx=\tilde R(p)$$Therefore:$$\large \tilde u(p,0)=A(p)e^0=A(p)=\tilde R(p)\implies \tilde u(p,t)=\tilde R(p)e^{(3ip-5)t}=e^{-5t}(\tilde R(p)e^{3ipt})$$Now using the shift theorem, we know that $\tilde R(x)e^{3ipt}$ is the FT of $R(x+3t)$, so we can say:$$\Huge u(x,t)=e^{-5t}R(x+3t)$$
We can also use this method to solve the IVP for the wave equation. Here, we have $u_{tt}=c^2u_{xx}$, $u(x,0)=R(x)$, and $u_t(x,0)=S(x)$. Taking FT:$$\Huge \tilde u_{tt}=c^2(ip)^2\tilde u=-c^2p^2\tilde u\implies\frac{\partial^2\tilde u}{\partial t^2}+c^2p^2\tilde u=0$$This is the equation for a simple harmonic oscillator, of which we know the solution:$$\Huge \tilde u(p,t)=A(p)\cos(pct)+B(p)\sin(pct)$$Now we use initial conditions to determine the functions in front of cos and sin:$$\Huge \tilde u(p,0)=A(p)=\int_{-\infty}^\infty u(x,0)e^{-ipx}dx=\int_{-\infty}^\infty R(x)e^{-ipx}dx=\tilde R(p)$$$$\Huge A(p)\cos(pct)=\tilde R(p)\left(\frac{1}{2}(e^{ipct}+e^{-ipct})\right)=\frac{1}{2}\tilde R(p)e^{ipct}+\frac{1}{2}\tilde R(p)e^{-ipct}$$Now applying the shift theorem gives:$$\Huge A(p)\cos(pct)=\frac{1}{2}R(x+ct)+\frac{1}{2}R(x-ct)$$
The other initial condition gives:$$\large \tilde u_t(p,0)=B(p)pc\cos(0)=B(p)pc=\int_{-\infty}^\infty u_t(x,0)e^{-ipx}dx=\int_{-\infty}^\infty S(x)e^{-ipx}dx=\tilde S(p)