
The position of a particle under quantum mechanics in one dimension is described by the function $\psi(x,t)$ that obeys the Schrodinger equation:$$\Huge i\hbar\frac{\partial\psi}{\partial t}=-\frac{\hbar^2}{2m}\frac{\partial^2\psi}{\partial x^2}+V(x)\psi$$This is first order in time, so to solve the IVP we need $\psi(x,0)=\psi(x)$. Here, $|\psi(x)|^2$ is a probability density of being measured at $x$. $\frac{1}{\sqrt{2\pi}}\tilde\psi(p)$ is the probability density for being measured with momentum $p$, where $\tilde\psi$ is the [[Fourier transform]] of $\psi$. $\Delta x$ is the standard deviation of probability density given by $|\psi|^2$, similarly with $\Delta p$. Heisenberg tells us:$$\Huge \Delta p\Delta x\geq\frac{\hbar}{2}$$Note that since $|\psi|^2$ is a probability density, it must integrate to one:$$\Huge \int_{-\infty}^\infty|\psi(x)|^2dx=1$$And also $\frac{1}{2\pi}|\tilde\psi|^2$ is a probability density so:$$\Huge \frac{1}{2\pi}\int_{-\infty}^\infty|\tilde\psi(p)|dp=1$$Then we can also say without loss of generality that:$$\Huge E(x)=\int_{-\infty}^\infty x|\psi(x)|^2dx=0,\,\,E(p)=\frac{1}{2\pi}\int_{-\infty}^\infty p|\tilde \psi(p)|^2dp=0$$This leads to the results:$$\Huge (\Delta x)^2=E(x^2)=\int_{-\infty}^\infty|\tilde\psi(x)|^2x^2dx,\,\,(\Delta p)^2=E(p^2)=\frac{1}{2\pi}\int_{-\infty}^\infty|\tilde \psi(p)|^2p^2dp$$Take for example $\psi(x)=\sqrt[4]{\frac{b}{\pi}}e^{-\frac{bx^2}{2}}$, making the FT $\tilde\psi(p)=\sqrt{2\pi}\sqrt[4]{\frac{1}{\pi b}}e^{-\frac{p^2}{2b}}$. We can then compute $(\Delta x)^2$:$$\Huge (\Delta x)^2=\int_{-\infty}^\infty|\psi(x)|^2x^2dx=\int_{-\infty}^\infty\sqrt{\frac{b}{\pi}}e^{-bx^2}x^2dx=\sqrt{\frac{b}{\pi}}\int_{-\infty}^\infty e^{-bx^2}x\,xdx$$$$\large (\Delta x)^2=\sqrt{\frac{b}{\pi}}\left[\frac{e^{-bx^2}}{-2b}x\right]_{-\infty}^\infty+\sqrt{\frac{b}{\pi}}\int_{-\infty}^\infty\frac{e^{-bx^2}}{2b}dx=0+\frac{1}{2\sqrt{\pi b}}\int_{-\infty}^\infty e^{-bx^2}dx=\frac{1}{2b}$$And also $(\Delta p)^2$:$$\Huge (\Delta p)^2=\frac{1}{2\pi}\int_{-\infty}^\infty|\tilde\psi(p)|^2p^2dp=\int_{-\infty}^\infty \frac{1}{\sqrt{\pi b}}e^{-\frac{p^2}{b}}p^2dp=\frac{b}{2}$$By a similar line of reasoning. We then get:$$\Huge (\Delta x)^2(\Delta p)^2=\frac{b}{2}\times\frac{1}{2b}=\frac{1}{4}\implies\Delta x\Delta p=\frac{1}{2}\geq\frac{\hbar }{2}$$So we have proven Heisenberg's uncertainty principle for this particular $\psi$. We now aim to prove it in the general case using Plancherel's Theorem, which states:$$\Huge \frac{1}{2\pi}\int_{-\infty}^\infty|\tilde\psi(p)|^2dp=\int_{-\infty}^\infty|\tilde \psi(x)|^2dx$$To prove this result look at the LHS:$$\large \frac{1}{2\pi}\int_{-\infty}^\infty|\tilde\psi(p)|^2dp=\frac{1}{2\pi}\int_{-\infty}^\infty\tilde\psi(p)\tilde\psi^*(p)dp=\frac{1}{2\pi}\int_{-\infty}^\infty\left(\int_{-\infty}^\infty\psi(x)e^{-ipx}dx\right)\tilde\psi^*(p)dp$$Using the definition of the FT, and using $*$ to denote the complex conjugate. However consider that if:$$\large \psi(x)=\frac{1}{2\pi}\int_{-\infty}^\infty\tilde\psi(p)e^{ipx}dp\implies\psi^*(x)=\frac{1}{2\pi}\int_{-\infty}^\infty(\tilde \psi(p)e^{ipx})^*dp=\frac{1}{2\pi}\int_{-\infty}^\infty\tilde\psi^*(p)e^{-ipx}dp$$We can then swap the order of the integration, keeping the $e^{-ipx}$ term, to use this:$$ \frac{1}{2\pi}\int_{-\infty}^\infty|\tilde\psi(p)|^2dp=\frac{1}{2\pi}\int_{-\infty}^\infty\psi(x)\left(\int_{-\infty}^\infty\tilde\psi^*(p)e^{-ipx}dp\right)dx=\frac{1}{2\pi}\int_{-\infty}^\infty\psi(x)(2\pi\,\psi^*(x))dx=\int_{-\infty}^\infty|\psi(x)|^2dx$$As required. Taking $F(x)=f'(x)$, observe that its FT is $\tilde F(p)=ip\tilde f(p)$. We can apply Plancherels theorem to this:$$\small \int_{-\infty}^\infty|\psi'(x)|^2dx=\int_{-\infty}^\infty|F(x)|^2=\frac{1}{2\pi}\int_{-\infty}^\infty|\tilde F(p)|^2dx=\frac{1}{2\pi}\int_{-\infty}^\infty|ip\,\tilde\psi(p)|^2=\frac{1}{2\pi}\int_{-\infty}^\infty p^2|\tilde \psi(p)|^2dp=E(p^2)=(\Delta p)^2$$Now we can prove the uncertainty principle by considering the following integral: