Given a [[Vector space definitions|vector space]] over $\Re$, a norm on $V$ is a function $||\cdot||:V\mapsto\Re$ such that:
> $||a\underline v||=|a|||\underline v||$, absolute homogeneity
> $||\underline u+\underline v||\leq||\underline u||+||\underline v||$, triangle inequality
> $||\underline v||=0\iff\underline v=\underline0$, separation of points

Using absolute homogeneity, observe that $||-\underline v||=||\underline v||$, making the triangle inequality:$$\Huge ||\underline v+(-\underline v)||=||0\cdot\underline v||=0\leq||\underline v||+||-\underline v||=2||\underline v||$$So we get that $||\underline v||\geq0$, non-negativity. When $V$ has an [[Inner product spaces|inner product]], there is a special norm induced by the inner product. In the real case, let $\{V,(\cdot,\cdot)\}$ be a real inner product space, then we let the norm induced by $(\cdot,\cdot)$ be defined by:$$\Huge ||\underline v||=\sqrt{(\underline v,\underline v)}\in\Re^+$$This is well defined since $(\underline v,\underline v)\geq0$ by definition. We define the unit vector if $||\underline v||=1$, and orthogonality if $(\underline u,\underline v)=0$, denoted as $\underline u\perp\underline v$.

We propose that if $\underline u\perp\underline v$ then:$$\Huge ||\underline u+\underline v||^2=||\underline u||^2+||\underline v||^2$$To prove this consider $||\underline u+\underline v||^2=(\underline u+\underline v,\underline u+\underline v)=(\underline u,\underline u)+2(\underline u,\underline v)+(\underline v,\underline v)=||\underline u||^2+0+0+||\underline v||^2$. Note also $||a\underline v||=\sqrt{(a\underline v,a\underline v)}=\sqrt{a^2(\underline v,\underline v)}=|a|||\underline v||$. So the definition of the norm induced by $(\cdot,\cdot)$ agrees with the definition of the norm.

# Cauchy-Schwarz inequality:

For a real inner product space $\{V,(\cdot,\cdot)\}$:$$\Huge (\underline u,\underline v)^2\leq(\underline u,\underline u)(\underline v,\underline v)$$The inequality becomes equality when $\underline u,\underline v$ are linearly dependent. We prove the above by first considering $\underline v=0$, in this case the proof is trivial so take $\underline v\neq0$ without loss of generality. Consider $\underline w=\underline u-\frac{(\underline u,\underline v)}{||\underline v||^2}\underline v$, then $0\leq||\underline w||^2=(\underline w,\underline w)=(\underline u-\frac{(\underline u,\underline v)}{||\underline v||^2}\underline v,\underline u-\frac{(\underline u,\underline v)}{||\underline v||^2}\underline v)=(\underline u,\underline u)-2\frac{(\underline u,\underline v)^2}{||\underline v||^2}+\frac{(\underline u,\underline v)^2(\underline v)}{}$