Let $R$ be a [[Rings, subrings, and fields|ring]]. A subset $I\subseteq R$ is called an ideal, $I$, of $R$ if it is closed under addition and for every $r\in R$ and $x\in I$ we have $r\cdot x\in I$ and $x\cdot r\in I$. Note that if $x\in I$, $0\cdot x=x\cdot 0\in I$, so $0\in I$ by default. Moreover $-1\cdot x\in I\implies -x\in I$. Note that if $1\in I$ then $I=R$ since for every $r\in R$ we have $1\cdot r=r\cdot 1\in I\implies r\in I$, so every element of $R$ is in $I$, and $I\subseteq R$, so $I=R$. 

This can be generalised to any unit in $R$. If $I\subseteq R$ is an ideal and $u\in I$ is a unit in $R$, then $I=R$. This comes from $u\in I\implies u^{-1}u\in I\implies 1\in I\implies I=R$. In a field $F$ the only ideals are the zero-ideal and $F$.

# Principle ideals:

For any commutative ring $R$ and $a\in R$ define the principle ideal generated by $a$:$$\Huge (a)=\{r\cdot a:r\in R\}$$Let $b,c\in(a)$, that is $b=r_1\cdot a$ and $c=r_2\cdot a$ for $r_1,r_2\in R$. Then $b+c=r_1a+r_2a=(r_1+r_2)a\in (a)$ since $r_1+r_2\in R$. Similarly for $r\in R,b\in(a)$ we have $r\cdot b=r\cdot(r_1a)=(r\cdot r_1)a\in (a)$ since $r\cdot r_1\in R$. 

Consider $a_1,a_2,\dots,a_n\in R$ and define:$$\Huge (a_1,\dots,a_n)=\{r_1\cdot a_1+\dots+r_n\cdot a_n:r_i\in R\}$$
Let $I_1=(a_1,\dots,a_m)$ and $I_2=(b_1,\dots,b_n)$ then $I_1=I_2$ if and only if $a_i\in I_2$ for $i=1,\dots,m$ and $b_j\in I$ for $j=1,\dots,n$. The forwards implication is trivial, so assume $a_i\in I_2$ for all $i=1,\dots,m$. Let $x\in I_1$, that is $x=r_1a_1+\dots+r_ma_m$ for some $r_i\in R$. However since $I_2$ is closed under addition we conclude $x\in I_2$ and say $I_1\subseteq I_2$. Similarly, one can show $I_2\subseteq I_1$, therefore $I_1=I_2$ as required.

For $n\in \mathbb{N}$ we consider $\varphi:\mathbb{Z}\mapsto \mathbb{Z}/n$ where $x\mapsto\bar x$. $x\in\ker\varphi$ if and only if $\bar x=\bar 0$, that is $n|x$ or $x=k\cdot n$ for some $k\in \mathbb{Z}$. Therefore $x\in (n)$, the principle ideal generated by $n$. Therefore, since $x$ was arbitrary we have $\ker\varphi=(n)$.

Consider the map $\varphi:\mathbb{Q}[x]\mapsto \mathbb{Q}$ with $f(x)\mapsto f(1)$. One can show that this is a ring [[Homomorphisms|homomorphism]]. Then we say $f(x)\in\ker\varphi\iff f(1)=0$. We claim that $\ker\varphi=(x-1)$, the principle ideal generated by $x-1$. We see that $(1)-1=0$ so $x-1\in\ker\varphi$, implying $(x-1)\subseteq\ker\varphi$. Let $f(x)\in\ker\varphi$ and write:$$\Huge f(x)=g(x)(x-1)+r(x)$$With $\deg r<1$. We then have $f(1)=0+r(x)=0+c=0\implies c=0\implies f(x)=g(x)(x-1)$. Therefore by definition $f(x)\in\ker\varphi\implies\ker\varphi\subseteq(x-1)$. We have subset both directions, so we can conclude $\ker\varphi=(x-1)$ indeed.

Given a ring $R$ and an ideal $I\subseteq R$, we ask if there exists a ring homomorphism $\varphi:R\mapsto S$ for some ring $S$ such that $\ker\varphi=I$. For $R=\mathbb{Z}$ and $I=(n)$ this is true since $\varphi:\mathbb{Z}\mapsto \mathbb{Z}/n$ gives $\ker\varphi=(n)$.

# Ideal equivalence relations:

We propose that if $\bar x,\bar y\in \mathbb{Z}/n$ then $x-y\in(n)$. Given a ring $R$ and an ideal $I$ we define an equivalence relation by $x=y\mod I$ if $x-y\in n$. We must check if this is reflexive, symmetric, and transitive:
> $x=x\mod I$ holds since $x-x=0\in I$, we have reflexivity
> Assuming $x=y\mod I, x-y\in I\implies -1(x-y)\in I\implies y-x\in I\implies y=x\mod I$, we have symmetry.
> Assume $x=y\mod I,y=z\mod I$. $x-y\in I,y-z\in I\implies x-y+y-z=x-z\in I\implies x=z\mod I$, we have transititivty.

This is indeed an equivalence relation.

# Cosets:

Let $I\subseteq R$ be an ideal in a ring $R$. Then for an $x\in R$ we define the coset of $I$ generated by $x$ to be the set:$$\Huge \bar x=x+I=\{x+r:r\in I\}\subseteq R$$
Let $x,y\in R$ and $I$ an ideal in $R$. Then the following are equivalent:
> $x+I=y+I$
> $x+I\cap y+I\neq\emptyset$
> $x-y\in I$

The first statement implies the second trivially. Since $x+I\cap y+I\neq\emptyset$ we have that $x+r=y+r'$ for some $r,r'\in I$. Then $x-y=r'-r\in I$ since $I$ is closed under addition, and we have that the second statement implies the third. $x-y\in I\implies x-y=r$ for some $r\in I$, therefore $x=y+r$. Notice $x+I=\{x+r':r'\in I\}=\{y+r+r':r,r'\in I\}=\{y+r:r\in I\}\subseteq y+I$, then we can write $y+I=\{y+r':r'\in I\}=\{x-r+r':r,r'\in I\}=\{x+r:r\in I\}\subseteq x+I$. We have both inclusions, so $x+I=y+I$. Therefore we have shown that the statements are a tautology.

# Rings modulo Ideals:

We can now define:$$\Huge R/I=\{x+I:x\in R\}=\{\bar x:x\in R\}$$This is the collection of all distinct cosets modulo $I$. We now define the following operations on this set:
> Addition: $(x+I)+(y+I):=x+y+I$
> Multiplication: $(x+I)(y+I):=xy+I$

To show that these [[Rings, subrings, and fields#Binary operations|binary operations]] are well defined, assume $x+I=x'+I$ and $y+I=y'+I$. Now we aim to show that $x+y+I=x'+y'+I$. We have that $x-x'\in I$ and $y-y'\in I$. This implies that $x-x'+y-y'\in I\implies x+y-(x'+y')\in I\implies x+y+I=x'+y'+I$. So addition is well defined. 

We now aim to show that if $x+I=x'+I$ and $y+I=y'+I$ then $xy+I=x'y'+I$. Since $x-x'\in R$ we have that $(x-x')y\in I$ and similarly since $y-y'\in I$ we have $x'(y-y')\in I$. Since the ideal is closed under addition we also have $(x-x')y+x'(y-y')=xy-x'y'\in I$. This is equivalent to saying $xy+I=x'y'+I$, so we have that multiplication is also well defined.

Hence on $R/I$ we have two well defined binary operations. The zero element is $0+I$ since $(x+I)+(0+I)=(x+0)+I=x+I$. The additive inverse of $x\in R/I$ is therefore $-(x+I)$ since $-(x+I)+(x+I)=(x-x)+I=0+I$. $1+I$ is the multiplicative identity since $(x+I)(1+I)=(x\cdot 1)+I=x+I$. One can also show associativity for both operations. Therefore $R/I$ is a ring.

Let $R$ be a ring and $I$ an ideal in $R$. Then the ring $R/I$ is called the quotient of $R$ by $I$, or $R\mod I$. It's elements $x+I=\bar x$ are called cosets, equivalence classes, or residue classes mod $I$. For example, if $I=R$ then there exists only one coset since $x+R=y+R$ as $x-y\in R$ always, that is $R/R=\{\bar 0\}$. Take $I=\{0\}$, then $R/I=R$ since for any two $x+I,y+I\in R/I$ $x-y=0\implies x=y$, so $x$ can be any element in $R$. Note that if $R$ is commutative, so is $R/I$.

Take $R=\mathbb{Q}[x]$ and $I=(x^2+x+1)=(g(x))$. Then $R/I=\{\bar p(x):p(x)\in \mathbb{Q}[x]\}=\{\bar r(x):\deg(r)\leq1\}$. Let $p(x)\in\mathbb{Q}[x]$, then $p(x)=q(x)g(x)+r(x)$ with $\deg(r)<\deg(g)=2$. Then $p(x)-r(x)=q(x)g(x)\in(g(x))=I$, therefore the equivalence class of $p$ and $r$ are identical. That is to say $\bar p(x)=\bar r(x)$. Note that if $r_1(x),r_2(x)$ are polynomials with degree less than or equal to $1$ and if $\bar r_1(x)=\bar r_2(x)$ then $r_1(x)-r_2(x)\in I\implies r_1(x)-r_2(x)=q(x)g(x)=0\implies r_1(x)=r_2(x)$. Take $p(x)=x^4-3x^2+2$, we aim to find $r(x)$ with $\deg(r)\leq1$ such that $p(x)=q(x)g(x)+r(x)$. Since $x^2+x+1\in I$ we have that $x^2+x+1-0\in I\implies\overline{x^2+x+1}=\bar 0\implies \bar x^2=\overline{-x-1}$. Now $\bar p(x)=\overline{x^4-3x^2+2}=\bar x^4+\overline{-3x^2+2}$. Notice $\bar x^4=\bar{(x^2)}^2=\overline{(-x-1)}^2$, expanding this gives $\bar x^2+\overline{2x}+\bar 1=\bar{-x}-\bar 1+\overline{2x}+\bar 1=\bar x$. Therefore $\bar p(x)=\bar x-3\overline{(-x-1)}+\bar 2=\overline{4x+5}$.

We can define the following ring homomorphism: $\pi:R\mapsto R/I$ with $x\mapsto\bar x$. This is indeed a ring homomorphism since:
> $\pi(1)=\bar 1$
> $\pi(x+y)=\overline(x+y)=\bar x+\bar y=\pi(x)+\pi(y)$
> $\pi(xy)=\overline{xy}=\bar x\cdot\bar y=\pi(x)\pi(y)$

We then aim to find the kernel of this map:$$\Huge\begin{align}
\ker\pi&=\{x\in R:\pi(x)=\bar 0\}\\
&= \{x\in R:\bar x=\bar 0\}\\
&=I
\end{align}$$
# First Isomorphism Theorem:

Let $\varphi:R\mapsto S$ be a ring homomorphism. Then the map defined as:$$\Huge\bar\varphi:R/\ker\varphi\mapsto\text{Im}(\varphi),\,\,\bar x\mapsto\varphi(x)$$Is a well defined ring homomorphism:$$\Huge R/\ker\varphi\cong\text{Im}(\varphi)$$To prove that this is well defined, let $x,x'\in R$ such that $\bar x=\bar x'$. Now we aim to show $\varphi(x)=\varphi(x')$. To do this, consider $\bar x=\bar x'\implies x-x'\in\ker\varphi\implies\varphi(x-x')=0\implies\varphi(x)-\varphi(x')=0\implies\varphi(x)=\varphi(x')$