Consider a particle of unit mass in a central force $f(r)=-\frac{1}{r^2}$. Starting at $r=1$ with initial speed $v_0$ and direction perpendicular to $\underline r$, we ask if we get a bounded orbit. Consider the potential energy:$$\Huge V(r)=-\int f(r)dr=-\int-\frac{1}{r^2}=-\frac{1}{r}$$And the total energy becomes:$$\Huge E=K+V=\frac{1}{2}v^2-\frac{1}{r}=_{t=0}\frac{1}{2}v_0^2-1$$As $r\to\infty$, then $E=\frac{1}{2}v^2-\frac{1}{r}\geq \frac{1}{r}\to0$. This implies at $t=0$, $\frac{1}{2}v_0^2-1\geq0$, and therefore $v_0\geq\sqrt{2}$. So we have that if $v_0<\sqrt{2}$ then $r(t)$ is bounded. To find the minimum and maximum values of $r$, consider [[Angular momentum and Central forces#Angular momentum|angular momentum]]: $$\Huge \underline L=m \underline r\times \underline{\dot r}=_{t=0}\underline e_r\times(v_0\underline e_\theta)=v_0\underline k\implies \underline L=v_0\implies\dot \theta=\frac{v_0}{r^2}$$So energy becomes:$$\Huge E=\frac{1}{2}(\dot r^2+r^2\dot \theta^2)-\frac{1}{r}=\frac{1}{2}\dot r^2+\frac{1}{2}v_0^2\frac{1}{r^2}-\frac{1}{r}$$However since this must be conserved, it is equal to initial conditions:$$\Huge \frac{1}{2}v_0^2-1=\frac{1}{2}\dot r^2+\frac{v_0^2}{2r^2}-\frac{1}{r}\implies \dot r^2+\frac{1}{r^2}(v_0^2-2r+(2-v_0^2)r^2)=0$$Take $v_0<\sqrt{2}$, we find min and max $r$ when $\dot r=0$. This gives solutions:$$\Huge r=1,\,\,r=\frac{v_0^2}{2-v_0^2}$$Whether each is a minimum or maximum is dependent on $v_0$. The range of possible $r$ then becomes $r\in\left[1,\frac{v_0^2}{2-v_0^2}\right]$. Note that if and only if the orbit is a circle, then $r_{\text{min}}=r_{\text{max}}$. This is true if and only if the following holds:$$\Huge \frac{v_0^2}{2-v_0^2}=r\iff v_0=1$$
# Finding the orbit:

We aim to find the orbit of an object in central force, in the form $r=r(\theta)$. It is often useful to use the variable $u=\frac{1}{r}$ instead of $r$, so we want to find an equation for $u(\theta)$. The chain rule gives:$$\Huge \frac{d}{dt}=\frac{Lu^2}{m}\frac{d}{d \theta}$$So we can write the following:$$\Huge \dot r=\frac{dr}{dt}=\frac{Lu^2}{m}\frac{d}{d \theta}\left(\frac{1}{u}\right)=-\frac{L}{m}u',\,\,\ddot r=\frac{d}{dt}\dot r=-\frac{L^2u^2}{m^2}u''$$Where $'$ is wrt to $\theta$. This makes the equation of motion:$$\Huge u''+u=-mL^{-2}u^{-2}f(u^{-1})$$This is the orbit equation,  a second order differential equation for $u(\theta)$. Take gravity as an example. Here we have $f(r)=-\frac{1}{r^2}$ and $m=1$. This makes the orbit equation:$$\Huge \frac{d^2u}{d \theta^2}+u=\frac{1}{L^2}\implies u(\theta)=A\cos(\theta-\theta_0)+\frac{1}{L^2}$$Rotating in polar coordinates to $\theta_0$ such that $\theta_0=0$ we can then write:$$\Huge r(\theta)=\frac{L^2}{1+\epsilon\cos\theta}$$Where $\epsilon>0$ is an arbitrary constant. Consider these cases:
> $\epsilon\in(0,1)$ causes the orbit to be bounded, since the denominator will never be $0$, making the curve an ellipse.
> $\epsilon>1$ causes the orbit to be unbounded, making the curve a hyperbola.
> $\epsilon=1$ causes the orbit to be unbounded, making the curve a parabola.

This parameter $\epsilon$ is called the eccentricity of the orbit.

# Circular orbits and stability:

For a circular orbit, an attractive force ($f(r)<0$) is required. Let us write $g(u)=-f(\frac{1}{u})$ so that $g$ is always positive. This makes the orbit equation:$$\Huge u''+u=\frac{mg(u)}{L^2u^2}$$A circular orbit where $u$ is constant is possible, with angular momentum satisfying $mg(b)=L^2b^3$ for some constant $b$. To determine if this is stable, we observe angular momentum. Take:$$\Huge u(\theta)=b+\epsilon(\theta)$$Substituting this into the orbit equation gives:$$\Huge \epsilon''+b+\epsilon=\frac{m}{L^2}(b+\epsilon)^{-2}g(b+\epsilon)\approx\frac{m}{L^2}b^{-2}(1-2b^{-1}\epsilon)(g(b)+\epsilon g'(b))$$Using Taylors theorem on $(b+ \epsilon)^{-2}$ and $g(b+\epsilon)$:$$\Huge \epsilon''+b+\epsilon\approx\frac{m}{L^2b^2}\left(g(b)+\left(g'(b)-\frac{2}{b}g(b)\right)\epsilon\right)$$$$\Huge \implies \epsilon''+\epsilon\approx\frac{m}{L^2b^2}\left(g'(b)-\frac{2}{b}g(b)\right)\epsilon$$Now using $\frac{m}{L^2b^2}=\frac{b}{g(b)}$:$$\Huge \epsilon''+\epsilon\approx\frac{bg'(b)}{g(b)}\epsilon-2\epsilon\implies \epsilon''+\left(3-\frac{bg'(b)}{g(b)}\right)\epsilon\approx0$$For $\epsilon(\theta)$ to stay small, we need the coefficient of $\epsilon$ in the above equation to be positive, as in simple harmonic motion. Therefore the orbit is stable if:$$\Huge 3-\frac{bg'(b)}{g(b)}>0\iff bg'(b)<3g(b)$$
Take gravity as an example ($f(r)=-\frac{1}{r^2}$):g(u)=u2⟹bg′(b)−3g(b)=2b3−3b2=−b2<0Therefore circular orbits under gravity are always stable. 

Example:  Consider a unit mass in $f(r)=-\frac{\alpha}{r^2}-\frac{\beta}{r^3}$ where $\alpha,\beta>0$. At time $t=0:(r, \theta)=(c,0)$ and speed is $\sqrt{\frac{4 \beta}{3c^2}}$ in a direction perpendicular to $\underline r$. Use $\frac{d^2u}{d \theta^2}+u=-\frac{1}{L^2u^2}f(u^{-1})$ to find $u(\theta)$ in terms of $\theta$ and constants. First we find $L$ using $\underline L=L \underline k= \underline r\times \underline{\dot r}=(c \underline e_r)\times(\sqrt{\frac{4 \beta}{3c^2}}\underline e_\theta)$ where $t=0$. Then we get $L=\sqrt{\frac{4 \beta}{3}}$. Now the orbit equation $u''+u=\frac{3}{4 \beta u^2}(\alpha u^2+ \beta u^3)=\frac{3 \alpha}{4 \beta}+\frac{3}{4}u\implies u''+\frac{1}{4}u=\frac{3 \alpha}{4 \beta}$. Now this is just a second order linear DE, which we solve to get the general solution $u=A\cos(\frac{1}{2}\theta)+B\sin(\frac{1}{2}\theta)+\frac{3 \alpha}{\beta}$. We can then determine $A,B$ by using $u(0)=\frac{1}{c}$ and $u'(0)=0$.