A mass $m$ is attatched to one end of a light rigid rod of length $Q$, the other end is attatched to a fixed point with the rod free to rotate in any direction. Gravity acts downwards with initial condition where the rod is horizontal, velocity is horizontal, and speed is $u$. We ask what distance $D$ below horizontal does the mass reach?
![[Spherical pendulum .excalidraw]]
Clearly when $g=0$, the mass does not swing downwards and we get [[Angular momentum and Central forces#Planar motion and Motion under central force|circular motion]] along the equator. When $u=0$ we get a simple pendulum and can determine that $D=Q$. We choose $z$ and $\underline k$ to be vertically downwards, and use polar coordinates along the horizontal. So we use $(r,\theta)$ with $(\underline e_r, \underline e_\theta)$, making the pivot at $z=0,r=0$. We write the position vector of the mass:$$\Huge \underline R=z \underline k+r \underline e_r$$Note that $\underline R\cdot \underline R=Q^2$, the distance from the origin is always $Q$. This implies that $\underline R\cdot\dot{\underline R}=0$ and $z^2+r^2=Q^2$:$$\Huge \underline{\dot R}=\dot z\underline k+\dot r\underline e_r+r\dot \theta\underline e_\theta$$Kinetic energy is:$$\Huge K=\frac{1}{2}mv^2=\frac{1}{2}m(\underline{\dot R}\cdot \underline{\dot R})=\frac{1}{2}m(\dot z^2+\dot r^2+r^2\dot \theta^2)$$We then claim that potential energy is:$$\Huge V=-mgz$$We look at the equation of motion to verify that total energy is conserved:$$\Huge m \underline{\ddot R}=mg \underline k+I$$Where $I$ is the tension along the rod, that is $I=h \underline R$ for some function $h$.$$\Huge \frac{dE}{dt}=m\underline{\dot R}\cdot\underline{\ddot R}-mg\dot z=\underline{\dot R}\cdot(mg \underline k+I)-mg\dot z$$Since $\underline R\cdot\underline{\dot R}=0$ , $I$ is proportional to $\underline R$, and $\underline{\dot R}\cdot \underline k=\dot z$ we get:$$\Huge \frac{dE}{dt}=0+mg\dot z-mg\dot z=0$$So we indeed have energy conserved. Our expressions are still very complex, so we aim to eliminate $\dot \theta^2$ by observing angular momentum $\underline L=m \underline R\times \underline{\dot R}$. However due to the additional gravitational force, angular momentum is not conserved as a vector. Not all hope is lost however, as we claim that the $\underline k$-component of angular momentum is conserved. That is, $\frac{dL_z}{dt}=\frac{d}{dt}(\underline L\cdot \underline k)=0$:$$\Huge \frac{dL_z}{dt}=m \frac{d}{dt}(\underline R\times \underline{\dot R})\cdot \underline k=m \underline R\times \underline{\ddot R}\cdot \underline k=\underline R\times(mg \underline k+I)\cdot \underline k=\underline 0+\underline R\times I\cdot \underline k$$Since $\underline R\times \underline k$ is orthogonal to $\underline k$, the LHS term in the triple product is $0$, and since $I$ is proportional to $\underline R$, the whole expression is $0$ and we get that the $\underline k$-component of angular momentum is conserved. Now:$$\large L_z=m \underline R\times \underline{\dot R}\cdot \underline k=m(z \underline k+r \underline e_r)\times(\dot z \underline k+\dot r \underline e_r+r \dot \theta \underline e_\theta)\cdot \underline k=mr^2\dot \theta \underline e_r\times \underline e_\theta\cdot \underline k=mr^2\dot \theta$$We can then apply initial conditions:$$\Huge L_z=mr(0)(r\dot \theta(0))=mQu$$$$\Huge E=\frac{1}{2}mu^2-mg\times0=\frac{1}{2}mu^2$$Now we aim to eliminate $\dot \theta$ and multiply energy by $\frac{2}{m}$:$$\Huge \frac{2}{m}E=\dot r^2+r^2\left(\frac{Qu}{r^2}\right)^2+\dot z^2-2gz=\dot r^2+\frac{Q^2u^2}{r^2}+\dot z^2-2gz=u^2$$We can now eliminate $\dot r$ by considering:$$\Huge \frac{d}{dt}(z^2+r^2)=\frac{d}{dt}(Q^2)\implies z\dot z+r\dot r=0\implies\dot r=-\frac{z\dot z}{r}$$This gives us:$$\Huge \frac{z^2\dot z^2}{r^2}+\frac{Q^2u^2}{r^2}+\dot z^2-2gz=u^2=\frac{z^2\dot z^2+Q^2u^2}{Q^2-z^2}+\dot z^2-2gz=u^2$$Now the only variable is $z$:$$\Huge z^2\dot z^2+Q^2u^2+(Q^2-z^2)(\dot z^2-2gz-u^2)=0$$This simplifies to:$$\Huge Q^2\dot z^2-2gz(Q^2-z^2)+u^2z^2=0\implies Q^2\dot z^2=H(z)$$Where $H(z)=2gQ^2z-2gz^3-u^2z^2$. This is now a first order separable differential equation. Since $\dot z^2\geq0$ we see that $H$ is restricted to $H(z)\geq0$. Crunching the numbers, we see that $H$ has zeros at $z=0$ and $z=\frac{1}{4g}(-u^2\pm\sqrt{u^4+16g^2Q^2})$. Since we begin at $z=0$, and there is a disallowed region between $0$ and the negative root, our allowed range of $z$ becomes:$$\Huge z\in[0,-u^2+\sqrt{u^4+16g^2Q^2}]$$